Coq: Clean up and update sketches

sketches/ArithExprCompiler.v
@@ -1,5 +1,8 @@
 (** Based on the arithmetic expression example in InductionExercises.v *)
 
+Set Implicit Arguments.
+Unset Strict Implicit.
+
 Require Import List PeanoNat.
 Import ListNotations Nat.
 
@@ -11,6 +14,12 @@ Inductive expr : Type :=
 | Modulo : expr -> expr -> expr
 | Ble    : expr -> expr -> expr
 | Beq    : expr -> expr -> expr.
+
+Infix "%+"  := Plus (left associativity, at level 50).
+Infix "%*"  := Times (left associativity, at level 45).
+Infix "%%"   := Modulo (left associativity, at level 51).
+Infix "%<=" := Ble (left associativity, at level 52).
+Infix "%="  := Beq (left associativity, at level 52).
 
 (** Reference evaluator -- denotational semantics *)
 Fixpoint eval_expr e :=
@@ -113,17 +122,12 @@ Fixpoint compile (e : expr) : prog :=
 
 (** Example expression and its compiled program *)
 Definition ex1   :=
-  Beq (Const 5)
-      (Plus (Const 1)
-            (Modulo (Plus (Const 9) (Plus (Plus (Const 1) (Const 3)) (Const 7))) (Const 5))).
+  (Const 9 %+ Const 1 %+ Const 3 %* Const 7 %% Const 9) %<= Const 9.
+Compute ex1.
 Definition prog1 := compile ex1.
 Definition res1  := run prog1 [].
 
 Compute (prog1, res1).
-Compute match list_eq_dec eq_dec res1 [eval_expr ex1] with
-        | left _  => true
-        | right _ => false
-        end.
 
 (** Correctness/correspondence theorem for stack compiler+evaluator *)
 Lemma run_app : forall p p' s, run (p ++ p') s = run p' (run p s).
@@ -136,10 +140,84 @@ Qed.
 
 Lemma compile_correct' : forall e s, run (compile e) s = eval_expr e :: s.
 Proof.
-  induction e; intro; cbn; solve [ reflexivity | now rewrite run_app, IHe2, run_app, IHe1 ].
+  induction e; intro; cbn;
+    solve [ reflexivity | now rewrite run_app, IHe2, run_app, IHe1 ].
 Qed.
 
 Theorem compile_correct : forall e, run (compile e) [] = [eval_expr e].
 Proof.
   now intro; rewrite compile_correct'.
 Qed.
+
+(** Operation small-step semantics for the language *)
+Reserved Infix "==>" (at level 60).
+Inductive step_expr : expr -> expr -> Prop :=
+(*| Step_Const : forall n, (* TODO: Should we have this? See also note below on [step_deterministic] *)
+    Const n ==> Const n*)
+
+| Step_Plus1 : forall e1 e1' e2,
+    e1 ==> e1' ->
+    e1 %+ e2 ==> e1' %+ e2
+| Step_Plus2 : forall n1 e2 e2',
+    e2 ==> e2' ->
+    Const n1 %+ e2 ==> Const n1 %+ e2'
+| Step_Plus3 : forall n1 n2,
+    Const n1 %+ Const n2 ==> Const (n1 + n2)
+
+| Step_Times1 : forall e1 e1' e2,
+    e1 ==> e1' ->
+    e1 %* e2 ==> e1' %* e2
+| Step_Times2 : forall n1 e2 e2',
+    e2 ==> e2' ->
+    Const n1 %* e2 ==> Const n1 %* e2'
+| Step_Times3 : forall n1 n2,
+    Const n1 %* Const n2 ==> Const (n1 * n2)
+
+| Step_Mod1 : forall e1 e1' e2,
+    e1 ==> e1' ->
+    e1 %% e2 ==> e1' %% e2
+| Step_Mod2 : forall n1 e2 e2',
+    e2 ==> e2' ->
+    Const n1 %% e2 ==> Const n1 %% e2'
+| Step_Mod3 : forall n1 n2,
+    Const n1 %% Const n2 ==> Const (n1 mod n2)
+
+| Step_Ble1 : forall e1 e1' e2,
+    e1 ==> e1' ->
+    e1 %<= e2 ==> e1' %<= e2
+| Step_Ble2 : forall n1 e2 e2',
+    e2 ==> e2' ->
+    Const n1 %<= e2 ==> Const n1 %<= e2'
+| Step_Ble3 : forall n1 n2,
+    Const n1 %<= Const n2 ==> Const (if n1 <=? n2 then 1 else 0)
+
+| Step_Beq1 : forall e1 e1' e2,
+    e1 ==> e1' ->
+    e1 %= e2 ==> e1' %= e2
+| Step_Beq2 : forall n1 e2 e2',
+    e2 ==> e2' ->
+    Const n1 %= e2 ==> Const n1 %= e2'
+| Step_Beq3 : forall n1 n2,
+    Const n1 %= Const n2 ==> Const (if n1 =? n2 then 1 else 0)
+where
+  "e1 '==>' e2" := (step_expr e1 e2).
+
+Require Import Relation_Operators.
+Definition step_expr_star := clos_refl_trans_1n _ step_expr.
+Notation "e1 '==>*' e2" := (step_expr_star e1 e2) (at level 60).
+
+(* TODO: Should we consider [==>] or [==>*]? *)
+Lemma step_deterministic : forall e, exists! n, e ==>* Const n.
+Proof.
+  induction e.
+  - exists n.
+    split; [ constructor; constructor | ].
+    inversion_clear 1; [ reflexivity | inversion H0 ].
+  - destruct IHe1 as [n1 [Hstep1 Hinv1]], IHe2 as [n2 [Hstep2 Hinv2]].
+    exists (n1 + n2).
+    split.
+    + inversion_clear Hstep1; inversion_clear Hstep2.
+      * econstructor; [ apply Step_Plus3 | constructor ].
+      * econstructor; [ apply Step_Plus2; eassumption | ].
+        fold step_expr_star in *.
+
