sketches/AxiomK.v
@@ -1,7 +1,6 @@
 Axiom K : forall {A} {x : A} (C : x = x -> Type),
   C eq_refl ->
-  forall loop : x = x,
-  C loop.
+  forall loop : x = x, C loop.
 
 Lemma all_refls :
   forall {A} {x : A} (p : x = x), p = eq_refl.
@@ -14,4 +13,6 @@ Qed.
 Goal forall {A} {x y : A} (p q : x = y), p = q.
 Proof.
   intros.
-  ???
+  destruct q.
+  apply all_refls.
+Qed.
