sketches/ListUtils.v
@@ -1,6 +1,0 @@
-Fixpoint last_error {A} (l : list A) :=
-  match l with
-  | cons x nil => Some x
-  | cons _ ys => last_error ys
-  | _ => None
-  end.
