sketches/ProgLang.v
@@ -1,0 +1,75 @@
+Set Implicit Arguments.
+
+Require Import List.
+Import ListNotations.
+
+Inductive type : Type :=
+| Nat  : type
+| Func : type -> type -> type.
+
+Inductive member (A : Type) (elm : A) : list A -> Type :=
+| HFirst : forall ls, member elm (elm :: ls)
+| HNext  : forall x ls, member elm ls -> member elm (x :: ls).
+
+Inductive term : list type -> type -> Type :=
+| Var   : forall G t, member t G -> term G t
+| Const : forall G, nat -> term G Nat
+| Plus  : forall G, term G Nat -> term G Nat -> term G Nat
+| Abs   : forall G dom ran,
+            term (dom :: G) ran -> term G (Func dom ran)
+| App   : forall G dom ran,
+            term G (Func dom ran) -> term G dom -> term G ran
+| Let   : forall G t1 t2,
+            term G t1 -> term (t1 :: G) t2 -> term G t2.
+
+Lemma ty_eq_dec : forall x y : type, {x = y} + {x <> y}.
+Proof. decide equality. Defined.
+
+Lemma term_case :
+  forall G t (P : term G t -> Type),
+    (forall p, P (Var p)) ->
+    (forall n (pf : t = Nat),
+        P (eq_rect Nat _ (Const G n) t (eq_sym pf))) ->
+    (forall e1 e2 (pf : t = Nat),
+        P (eq_rect Nat _ (Plus e1 e2) t (eq_sym pf))) ->
+    (forall dom ran (pf : t = Func dom ran) b,
+        P (eq_rect (Func dom ran) _ (Abs b) _ (eq_sym pf))) ->
+    (forall dom e1 e2, P (App (dom:=dom) e1 e2)) ->
+    (forall ty1 e1 e2, P (Let (t1:=ty1) e1 e2)) ->
+    forall e, P e.
+Proof.
+  intros.
+  destruct e eqn:?; auto.
+  - specialize (X0 n eq_refl); auto.
+  - specialize (X1 t0_1 t0_2 eq_refl); auto.
+  - specialize (X2 dom ran eq_refl t0); auto.
+Qed.
+
+Ltac term_destruct v :=
+  pattern v; apply term_case; clear v; intros.
+
+Fixpoint cfold G t (e : term G t) : term G t :=
+    match e with
+      | @Plus G e1 e2 =>
+        let e1' := cfold e1 in
+        let e2' := cfold e2 in
+        let maybeOpt := match e1' return _ with
+                          | Const _ n1 =>
+                            match e2' return _ with
+                              | Const _ n2 => Some (@Const G (n1 + n2))
+                              | _ => None
+                            end
+                          | _ => None
+                        end in
+        match maybeOpt with
+          | None    => Plus e1' e2'
+          | Some e' => e'
+        end
+
+      | Abs e1    => Abs (cfold e1)
+      | App e1 e2 => App (cfold e1) (cfold e2)
+
+      | Let e1 e2 => Let (cfold e1) (cfold e2)
+
+      | e => e
+    end.
